src/utils.c
@@ -10,6 +10,6 @@ C_String_t Utils_topic_name_uint8_to_c_string(uint8_t *u8_buffer) {
   return (char *)u8_buffer;
 }
 
-C_String_t Utils_payload_uint8_to_c_string(uint8_t *u8_buffer, uint32_t n) {
+C_String_t Utils_payload_uint8_to_c_string(uint8_t *u8_buffer, uint32_t min_packet_size, uint32_t max_packet_size, uint32_t n) {
   return (char *)u8_buffer;
 }
